Imp/Expr/Optimize.lean
@@ -19,6 +19,11 @@ def opOpt : BinOp → Expr → Expr → Expr
   | .plus, e, const 0 => e
   | .times, .const 1, e => e
   | .times, e, const 1 => e
+  | .times, .const 0, e2' =>
+    if e2'.hasNoDiv then
+      .const 0
+    else
+      .op .times (.const 0) e2'
   | bop, e1, e2 => .op bop e1 e2
 
 /--
@@ -37,10 +42,22 @@ theorem unopOpt_ok : (Expr.unopOpt uop e).eval σ = (Expr.unop uop e).eval σ :=
   split <;> simp [eval, *]
   · split <;> simp [eval, *]
 
+-- omission in the stdlib
+@[simp] theorem BitVec_0_mul : 0#32 * v = 0#32 := by rw [BitVec.mul_comm]; simp
+
+-- simplification rules for `BinOp.apply`
 @[simp] theorem BinOp.apply_plus_0_left  : BinOp.plus.apply (0#32) v = v := by simp [BinOp.apply]
 @[simp] theorem BinOp.apply_plus_0_right : BinOp.plus.apply v (0#32) = v := by simp [BinOp.apply]
 @[simp] theorem BinOp.apply_mul_1_left   : BinOp.times.apply (1#32) v = v := by simp [BinOp.apply]
 @[simp] theorem BinOp.apply_mul_1_right  : BinOp.times.apply v (1#32) = v := by simp [BinOp.apply]
+@[simp] theorem BinOp.apply_mul_0_left   : BinOp.times.apply (0#32) v = 0#32 := by simp [BinOp.apply]
+@[simp] theorem BinOp.apply_mul_0_right  : BinOp.times.apply v (0#32) = 0#32 := by simp [BinOp.apply]
+
+/-- Helper lemma to deal with `Option.isSome` -/
+theorem Option.bind_const_of_isSome (h : o.isSome) : Option.bind o (fun _ => x) = x := by
+  cases o
+  · simp at h
+  · simp
 
 /-- Correctness of the `.opOpt` smart constructor -/
 @[simp]
@@ -48,7 +65,8 @@ theorem opOpt_ok : (Expr.opOpt bop e1 e2).eval σ = (Expr.op bop e1 e2).eval σ 
   unfold Expr.opOpt
   split <;> simp [eval, *]
   · split <;> simp [eval, *]
-
+  next bop e1 e2 =>
+    split <;> simp [eval, eval_isSome_of_hasDiv, Option.bind_const_of_isSome, *]
 /--
 Optimization doesn't change the meaning of any expression
 -/
